%% LyX 2.3.6.1 created this file.  For more info, see http://www.lyx.org/.
%% Do not edit unless you really know what you are doing.
\documentclass[english]{article}
\usepackage[T1]{fontenc}
\usepackage[latin9]{inputenc}
\setlength{\parindent}{0bp}
\usepackage{amstext}
\usepackage{wasysym}
\usepackage{babel}
\begin{document}
\begin{itemize}
\item Ex.1 
\end{itemize}

\paragraph{1)}

\paragraph{We know that :}

\paragraph{$Var(x)=E[x^{2}]-E[x]^{2}=\sigma^{2}$ (1) }

\paragraph{$\frac{1}{n}\mathord{\mathop{\sum^{n}{\scriptscriptstyle \iota=1}\mathord{x{\scriptscriptstyle i}}}}=M$
(2)}

\paragraph{$\frac{1}{n}\mathord{\mathop{\sum^{n}{\scriptscriptstyle \iota=1}(\mathord{x{\scriptscriptstyle i}}-M)^{2}}=\frac{1}{n}\mathord{\mathop{\sum^{n}{\scriptscriptstyle \iota=1}\mathord{x{\scriptscriptstyle i}^{2}}-nM^{2}}}}$(3)}

\paragraph{$E[M]=\text{\ensuremath{\mu}}$(4)}

\paragraph{$Var(M)=\sigma^{2}$}

\paragraph{Starting from:}

\paragraph{$W{\scriptscriptstyle n}^{2}=\frac{1}{n}\mathord{\mathop{\sum^{n}{\scriptscriptstyle \iota=1}(\mathord{x{\scriptscriptstyle i}}-\mu)^{2}}}$}

\paragraph{We can say that:}

\paragraph{$E[W{\scriptscriptstyle n}^{2}]=E[\frac{1}{n}\mathord{\mathop{\sum^{n}{\scriptscriptstyle \iota=1}(\mathord{x{\scriptscriptstyle i}}-\mu)^{2}}]=\frac{1}{n}\mathord{\mathop{\sum^{n}{\scriptscriptstyle \iota=1}E[(\mathord{x{\scriptscriptstyle i}}-\mu)^{2}}]=}}$}

\paragraph*{$=\frac{1}{n}\mathord{\mathop{\sum^{n}{\scriptscriptstyle \iota=1}(E[\mathord{x{\scriptscriptstyle i^{2}}}]-2E[\mu x{\scriptscriptstyle i}]+E[\mu^{2}}])=\frac{1}{n}\mathord{\mathop{\sum^{n}{\scriptscriptstyle \iota=1}(E[\mathord{x{\scriptscriptstyle i^{2}}}]-2\mu E[x{\scriptscriptstyle i}])+n\mu^{2}}=}}$}

\paragraph{$=\frac{1}{n}\mathord{\mathop{(\sum^{n}{\scriptscriptstyle \iota=1}E[\mathord{x{\scriptscriptstyle i^{2}}}]-2n\mu^{2}+n\mu^{2})}=}$}

\paragraph{$=\frac{1}{n}\mathord{\mathop{(n\sigma^{2}+n\mu^{2}-2n\mu^{2}+n\mu^{2}})=}\sigma^{2}$}

\paragraph{which proves that $W{\scriptscriptstyle n}^{2}$is unbiased estimator
of $\sigma^{2}$}

\paragraph{Now starting from:}

\paragraph{$S{\scriptscriptstyle n}^{2}=\frac{1}{n-1}\mathord{\mathop{\sum^{n}{\scriptscriptstyle \iota=1}(\mathord{x{\scriptscriptstyle i}}-\frac{1}{n}\mathord{\mathop{\Sigma^{n}{\scriptscriptstyle \iota=1}\mathord{x{\scriptscriptstyle i}}}})^{2}}}$}

\paragraph{We can say that:}

\paragraph{$E[S{\scriptscriptstyle n}^{2}]=E[\mathord{\mathop{\frac{1}{n-1}\mathord{\mathop{\sum^{n}{\scriptscriptstyle \iota=1}(\mathord{x{\scriptscriptstyle i}}-\frac{1}{n}\mathord{\mathop{\sum^{n}{\scriptscriptstyle \iota=1}\mathord{x{\scriptscriptstyle i}}}})^{2}}}}]=\frac{1}{n-1}\mathord{\mathop{\sum^{n}{\scriptscriptstyle \iota=1}E[(\mathord{x{\scriptscriptstyle i}}-M)^{2}}]}}$}

\paragraph{from (3)}

\paragraph{$\frac{1}{n-1}\mathord{\mathop{\sum^{n}{\scriptscriptstyle \iota=1}E[(\mathord{x{\scriptscriptstyle i}}-M)^{2}}]}=\frac{1}{n-1}\mathord{\mathop{\sum^{n}{\scriptscriptstyle \iota=1}\mathord{E[x{\scriptscriptstyle i}^{2}]}-nE[M^{2}]}}=$}

\paragraph*{$=\frac{1}{n-1}\mathord{\mathop{\sum^{n}{\scriptscriptstyle \iota=1}E[\mathord{x{\scriptscriptstyle i}^{2}}]-\frac{n}{n-1}(\mu^{2}+\frac{\sigma^{2}}{n}})=\frac{n}{n-1}\mathord{\mathop{(\sigma^{2}+\mu^{2})-\frac{n}{n-1}(}\frac{\sigma^{2}}{n}+\mu^{2})=\sigma^{2}}}$}

\paragraph{which proves that $S{\scriptscriptstyle n}^{2}$is also unbiased
estimator of $\sigma^{2}$}

\paragraph*{2) }

\paragraph*{To prove that $(W{\scriptscriptstyle n}^{2})^{\wasypropto}{\scriptscriptstyle i=1}$,
$(S{\scriptscriptstyle n}^{2})^{\wasypropto}{\scriptscriptstyle i=2}$
are consistent we should prove that $Var((W{\scriptscriptstyle n}^{2})^{\wasypropto}{\scriptscriptstyle i=1})$
and $Var((S{\scriptscriptstyle n}^{2})^{\wasypropto}{\scriptscriptstyle i=2})$
are almost zero, as n approximates infinity}

\paragraph*{and this is true because:}

\paragraph*{$Var((W{\scriptscriptstyle n}^{2})^{\wasypropto}{\scriptscriptstyle i=1})=\frac{1}{n}\mathord{\mathop{\sum^{n}{\scriptscriptstyle \iota=1}Var(\mathord{x{\scriptscriptstyle i}}-\mu)^{2}}}$}

\paragraph*{$Var(S{\scriptscriptstyle n}^{2})=\frac{1}{n-1}\mathord{\mathop{\sum^{n}{\scriptscriptstyle \iota=1}Var((\mathord{x{\scriptscriptstyle i}}-\frac{1}{n}\mathord{\mathop{\Sigma^{n}{\scriptscriptstyle \iota=1}\mathord{x{\scriptscriptstyle i}}}})^{2})}}$}

\paragraph*{as n approximates infinity $\frac{1}{n}$ becomes zero so both of
them are equal to zero}

\paragraph*{3)}

\paragraph*{To prove that $W{\scriptscriptstyle n}^{2}=\frac{1}{n}\mathord{\mathop{\sum^{n}{\scriptscriptstyle \iota=1}(\mathord{x{\scriptscriptstyle i}}-\mu)^{2}}}$
is more efficient that $S{\scriptscriptstyle n}^{2}=\frac{1}{n-1}\mathord{\mathop{\sum^{n}{\scriptscriptstyle \iota=1}(\mathord{x{\scriptscriptstyle i}}-\frac{1}{n}\mathord{\mathop{\Sigma^{n}{\scriptscriptstyle \iota=1}\mathord{x{\scriptscriptstyle i}}}})^{2}}}$
we should prove that $Var(W{\scriptscriptstyle n}^{2})\prec$$Var(S{\scriptscriptstyle n}^{2})$ }

\paragraph*{as we already proved ,they are both unbiased estimators of $\sigma^{2}$}

\paragraph*{$Var(W{\scriptscriptstyle n}^{2})=\frac{1}{n}\mathord{\mathop{\Sigma^{n}{\scriptscriptstyle \iota=1}Var(\mathord{x{\scriptscriptstyle i}}-\mu)^{2}}}=$$\frac{1}{n}(\sigma{\scriptscriptstyle 4}-\sigma^{4})$ }

\paragraph*{$Var(S{\scriptscriptstyle n}^{2})=\frac{1}{n-1}\mathord{\mathop{\sum^{n}{\scriptscriptstyle \iota=1}Var((\mathord{x{\scriptscriptstyle i}}-\frac{1}{n}\mathord{\mathop{\Sigma^{n}{\scriptscriptstyle \iota=1}\mathord{x{\scriptscriptstyle i}}}})^{2})}}$}

\paragraph*{knowing that:}

\paragraph*{$S{\scriptscriptstyle n}^{2}=\frac{1}{2n(n-1)}\sum^{n}{\scriptscriptstyle \iota=1}\sum^{n}{\scriptscriptstyle j=1}(x{\scriptscriptstyle i}-x{\scriptscriptstyle j})$}

\paragraph*{$Var(S{\scriptscriptstyle n}^{2})=Cov(S{\scriptscriptstyle n}^{2},S{\scriptscriptstyle n}^{2})=\frac{1}{4n^{2}(n-1)^{2}}\sum^{n}{\scriptscriptstyle \iota=1}\sum^{n}{\scriptscriptstyle j=1}\sum^{n}{\scriptscriptstyle k=1}\sum^{n}{\scriptscriptstyle l=1}(x{\scriptscriptstyle i}-x{\scriptscriptstyle j})^{2}(x{\scriptscriptstyle k}-x{\scriptscriptstyle l})^{2}$}

\paragraph*{We have four cases:}

\paragraph*{$2n^{3}-n^{2}$ terms if $Cov((x{\scriptscriptstyle i}-x{\scriptscriptstyle j})^{2}(x{\scriptscriptstyle k}-x{\scriptscriptstyle l})^{2})=0$
if i=j or k=l}

\paragraph*{$n(n-1)(n-2)(n-3)$ terms if $Cov((x{\scriptscriptstyle i}-x{\scriptscriptstyle j})^{2}(x{\scriptscriptstyle k}-x{\scriptscriptstyle l})^{2})=0$
if i,j,k are distinct}

\paragraph*{$2n(n-1)$ terms if $Cov((x{\scriptscriptstyle i}-x{\scriptscriptstyle j})^{2}(x{\scriptscriptstyle k}-x{\scriptscriptstyle l})^{2})=2\sigma{\scriptscriptstyle 4}-2\sigma^{4}$
if i!=j and \{k,l\}=\{i,j\}}

\paragraph*{$4n(n-1)(n-2)$ terms if $Cov((x{\scriptscriptstyle i}-x{\scriptscriptstyle j})^{2}(x{\scriptscriptstyle k}-x{\scriptscriptstyle l})^{2})=\sigma{\scriptscriptstyle 4}-\sigma^{4}$
if i!=j and k!=l and $|(\{i,j\}\land\{k,l\})|$}

\paragraph*{Substituting gives the result:}

\paragraph*{$Var(S{\scriptscriptstyle n}^{2})=\frac{1}{n}(\sigma{\scriptscriptstyle 4}-\frac{n-3}{n-1}\sigma^{4})$}

\paragraph*{$Var(S{\scriptscriptstyle n}^{2})-Var(W{\scriptscriptstyle n}^{2})=\frac{1}{n}(\sigma{\scriptscriptstyle 4}-\frac{n-3}{n-1}\sigma^{4})-\frac{1}{n}(\sigma{\scriptscriptstyle 4}-\sigma^{4})=\sigma{\scriptscriptstyle 4}-\sigma^{4}\succ0$}

\paragraph*{$Var(S{\scriptscriptstyle n}^{2})\succ Var(W{\scriptscriptstyle n}^{2})$}

\paragraph*{4)}

\paragraph*{The asymptotic relative efficient of $W{\scriptscriptstyle n=1}^{2}$to$S{\scriptscriptstyle n=2}^{2}$is:}

\paragraph*{$lim{\scriptscriptstyle n\rightarrow\wasypropto}(Eff(W{\scriptscriptstyle n=1}^{2}t,S{\scriptscriptstyle n=2}^{2}))=lim{\scriptscriptstyle n\rightarrow\wasypropto}(\frac{Var(S{\scriptscriptstyle n}^{2})}{Var(W{\scriptscriptstyle n})})=lim{\scriptscriptstyle n\rightarrow\wasypropto}(\frac{\frac{1}{n}(\sigma{\scriptscriptstyle 4}-\frac{n-3}{n-1}\sigma^{4})}{\frac{1}{n}(\sigma{\scriptscriptstyle 4}-\sigma^{4})})=lim{\scriptscriptstyle n\rightarrow\wasypropto}\frac{(n-1)\sigma{\scriptscriptstyle 4}-(n-3)\sigma^{4}}{(n-1)(\sigma{\scriptscriptstyle 4}-\sigma^{4})}=1$ }
\end{document}
